%Dimostrazione per Induzione esempio 6
\begin{thm}
    $\displaystyle \sum _{k=1} ^ n k^3 = \frac{n^2 (n+1)^2}{4}$
\end{thm}

%Dimostrazione
\begin{proof}
Caso base: $n = 1 \sum _{k=1} ^ 1 k^3 = \frac{1^2(1+1)^2}{4} 1 = \frac{4}{4} \text{vero}$

Ipotesi induttiva: $\sum _{k=1} ^ n k^3 = \frac{n^2 (n+1)^2}{4}$
Tesi induttiva: $\sum _{k=1} ^ {n+1} k^3 = \frac{(n+1)^2 (n+2)^2}{4}$
\begin{equation*}
\begin{split}
\sum _{k=1} ^{n+1} k^3 & = \sum _{k=1} ^ n k^3 + (n+1)^3 \\
                       & = \frac{n^2 (n+1)^2}{4} + (n+1)^3 \\
                       & = (n+1)^2 (\frac{n^2}{4} + (n+1)) \\
                       & = (n+1)^2 (\frac{n^2 + 4n + 4}{4}) \\
                       & = \frac{(n+1)^2 (n+2)^2}{4} \\
\end{split}
\end{equation*}
\end{proof}
